thys/JinjaThreads/Compiler/Correctness1Threaded.thy
@@ -13,8 +13,8 @@ definition lock_oks1 ::
   "('addr,'thread_id) locks 
   \<Rightarrow> ('addr,'thread_id,(('a,'b,'addr) exp \<times> 'c) \<times> (('a,'b,'addr) exp \<times> 'c) list) thread_info \<Rightarrow> bool" 
 where
-  "lock_oks1 ls ts \<equiv> \<forall>t. (case (ts t) of None    \<Rightarrow> (\<forall>l. has_locks (ls\<^sub>f l) t = 0)
-                            | \<lfloor>((ex, exs), ln)\<rfloor> \<Rightarrow> (\<forall>l. has_locks (ls\<^sub>f l) t + ln\<^sub>f l = expr_lockss (map fst (ex # exs)) l))"
+  "lock_oks1 ls ts \<equiv> \<forall>t. (case (ts t) of None    \<Rightarrow> (\<forall>l. has_locks (ls $ l) t = 0)
+                            | \<lfloor>((ex, exs), ln)\<rfloor> \<Rightarrow> (\<forall>l. has_locks (ls $ l) t + ln $ l = expr_lockss (map fst (ex # exs)) l))"
 
 primrec el_loc_ok :: "'addr expr1 \<Rightarrow> 'addr locals1 \<Rightarrow> bool"
   and els_loc_ok :: "'addr expr1 list \<Rightarrow> 'addr locals1 \<Rightarrow> bool"
@@ -129,21 +129,21 @@ apply(auto simp add: is_vals_conv intro: ext)
 done
 
 lemma lock_oks1I:
-  "\<lbrakk> \<And>t l. ts t = None \<Longrightarrow> has_locks (ls\<^sub>f l) t = 0;
-     \<And>t e x exs ln l. ts t = \<lfloor>(((e, x), exs), ln)\<rfloor> \<Longrightarrow> has_locks (ls\<^sub>f l) t + ln\<^sub>f l= expr_locks e l + expr_lockss (map fst exs) l \<rbrakk>
+  "\<lbrakk> \<And>t l. ts t = None \<Longrightarrow> has_locks (ls $ l) t = 0;
+     \<And>t e x exs ln l. ts t = \<lfloor>(((e, x), exs), ln)\<rfloor> \<Longrightarrow> has_locks (ls $ l) t + ln $ l= expr_locks e l + expr_lockss (map fst exs) l \<rbrakk>
   \<Longrightarrow> lock_oks1 ls ts"
 apply(fastforce simp add: lock_oks1_def)
 done
 
 lemma lock_oks1E:
   "\<lbrakk> lock_oks1 ls ts;
-     \<forall>t. ts t = None \<longrightarrow> (\<forall>l. has_locks (ls\<^sub>f l) t = 0) \<Longrightarrow> Q;
-     \<forall>t e x exs ln. ts t = \<lfloor>(((e, x), exs), ln)\<rfloor> \<longrightarrow> (\<forall>l. has_locks (ls\<^sub>f l) t + ln\<^sub>f l = expr_locks e l + expr_lockss (map fst exs) l) \<Longrightarrow> Q \<rbrakk>
+     \<forall>t. ts t = None \<longrightarrow> (\<forall>l. has_locks (ls $ l) t = 0) \<Longrightarrow> Q;
+     \<forall>t e x exs ln. ts t = \<lfloor>(((e, x), exs), ln)\<rfloor> \<longrightarrow> (\<forall>l. has_locks (ls $ l) t + ln $ l = expr_locks e l + expr_lockss (map fst exs) l) \<Longrightarrow> Q \<rbrakk>
   \<Longrightarrow> Q"
 by(fastforce simp add: lock_oks1_def)
 
 lemma lock_oks1D1:
-  "\<lbrakk> lock_oks1 ls ts; ts t = None \<rbrakk> \<Longrightarrow> \<forall>l. has_locks (ls\<^sub>f l) t = 0"
+  "\<lbrakk> lock_oks1 ls ts; ts t = None \<rbrakk> \<Longrightarrow> \<forall>l. has_locks (ls $ l) t = 0"
 apply(simp add: lock_oks1_def)
 apply(erule_tac x="t" in allE)
 apply(auto)
@@ -151,7 +151,7 @@ done
 
 lemma lock_oks1D2:
   "\<lbrakk> lock_oks1 ls ts; ts t = \<lfloor>(((e, x), exs), ln)\<rfloor> \<rbrakk> 
-  \<Longrightarrow> \<forall>l. has_locks (ls\<^sub>f l) t + ln\<^sub>f l = expr_locks e l + expr_lockss (map fst exs) l"
+  \<Longrightarrow> \<forall>l. has_locks (ls $ l) t + ln $ l = expr_locks e l + expr_lockss (map fst exs) l"
 apply(fastforce simp add: lock_oks1_def)
 done
 
@@ -271,9 +271,9 @@ proof(intro ext iffI)
     assume "\<exists>l. ta = \<lbrace>UnlockFail\<rightarrow>l\<rbrace> \<and> 0 < expr_lockss (fst ex # map fst exs) l"
     then obtain l where ta: "ta = \<lbrace>UnlockFail\<rightarrow>l\<rbrace>" 
       and el: "expr_lockss (fst ex # map fst exs) l > 0" by blast
-    from aoe have "lock_actions_ok ((locks s)\<^sub>f l) t (\<lbrace>ta\<rbrace>\<^bsub>l\<^esub>\<^sub>f l)"
+    from aoe have "lock_actions_ok (locks s $ l) t (\<lbrace>ta\<rbrace>\<^bsub>l\<^esub> $ l)"
       by(auto simp add: lock_ok_las_def)
-    with ta have "has_locks ((locks s)\<^sub>f l) t = 0" by simp
+    with ta have "has_locks (locks s $ l) t = 0" by simp
     with lok tst have "expr_lockss (map fst (ex # exs)) l = 0"
       by(cases ex)(auto 4 6 simp add: lock_oks1_def)
     with el have False by simp
@@ -395,34 +395,34 @@ proof(cases rule: Red1_mthr.redT.cases)
     { fix t'
       assume None: "(redT_updTs (thr s1) (map (convert_new_thread_action (extNTA2J1 P)) \<lbrace>TA\<rbrace>\<^bsub>t\<^esub>)(t \<mapsto> (((e', x'), exs), redT_updLns (locks s1) t (snd (the (thr s1 t))) \<lbrace>TA\<rbrace>\<^bsub>l\<^esub>))) t' = None"
       { fix l
-	from aoe have "lock_actions_ok ((locks s1)\<^sub>f l) t (\<lbrace>ta\<rbrace>\<^bsub>l\<^esub>\<^sub>f l)" by(auto simp add: lock_ok_las_def)
-	with None have "has_locks ((redT_updLs (locks s1) t \<lbrace>ta\<rbrace>\<^bsub>l\<^esub>)\<^sub>f l) t' = has_locks ((locks s1)\<^sub>f l) t'"
+	from aoe have "lock_actions_ok (locks s1 $ l) t (\<lbrace>ta\<rbrace>\<^bsub>l\<^esub> $ l)" by(auto simp add: lock_ok_las_def)
+	with None have "has_locks ((redT_updLs (locks s1) t \<lbrace>ta\<rbrace>\<^bsub>l\<^esub>) $ l) t' = has_locks (locks s1 $ l) t'"
 	  by(auto split: split_if_asm)
-	also from loks None have "has_locks ((locks s1)\<^sub>f l) t' = 0" unfolding lock_oks1_def
+	also from loks None have "has_locks (locks s1 $ l) t' = 0" unfolding lock_oks1_def
 	  by(force split: split_if_asm dest!: redT_updTs_None)
-	finally have "has_locks (upd_locks ((locks s1)\<^sub>f l) t (\<lbrace>TA\<rbrace>\<^bsub>l\<^esub>\<^sub>f l)) t' = 0" by simp }
-      hence "\<forall>l. has_locks (upd_locks ((locks s1)\<^sub>f l) t (\<lbrace>TA\<rbrace>\<^bsub>l\<^esub>\<^sub>f l)) t' = 0" .. }
+	finally have "has_locks (upd_locks (locks s1 $ l) t (\<lbrace>TA\<rbrace>\<^bsub>l\<^esub> $ l)) t' = 0" by simp }
+      hence "\<forall>l. has_locks (upd_locks (locks s1 $ l) t (\<lbrace>TA\<rbrace>\<^bsub>l\<^esub> $ l)) t' = 0" .. }
     moreover {
       fix t' eX eXS LN
       assume Some: "(redT_updTs (thr s1) (map (convert_new_thread_action (extNTA2J1 P)) \<lbrace>TA\<rbrace>\<^bsub>t\<^esub>)(t \<mapsto> (((e', x'), exs), redT_updLns (locks s1) t (snd (the (thr s1 t))) \<lbrace>TA\<rbrace>\<^bsub>l\<^esub>))) t' = \<lfloor>((eX, eXS), LN)\<rfloor>"
       { fix l
-	from aoe have lao: "lock_actions_ok ((locks s1)\<^sub>f l) t (\<lbrace>ta\<rbrace>\<^bsub>l\<^esub>\<^sub>f l)" by(auto simp add: lock_ok_las_def)
-	have "has_locks ((redT_updLs (locks s1) t \<lbrace>ta\<rbrace>\<^bsub>l\<^esub>)\<^sub>f l) t' + LN\<^sub>f l = expr_lockss (map fst (eX # eXS)) l"
+	from aoe have lao: "lock_actions_ok (locks s1 $ l) t (\<lbrace>ta\<rbrace>\<^bsub>l\<^esub> $ l)" by(auto simp add: lock_ok_las_def)
+	have "has_locks ((redT_updLs (locks s1) t \<lbrace>ta\<rbrace>\<^bsub>l\<^esub>) $ l) t' + LN $ l = expr_lockss (map fst (eX # eXS)) l"
 	proof(cases "t = t'")
 	  case True
 	  from loks thrst x
-	  have "has_locks ((locks s1)\<^sub>f l) t = expr_locks e l + expr_lockss (map fst exs) l"
+	  have "has_locks (locks s1 $ l) t = expr_locks e l + expr_lockss (map fst exs) l"
 	    by(force simp add: lock_oks1_def)
-	  hence "lock_expr_locks_ok ((locks s1)\<^sub>f l) t 0 (int (expr_locks e l + expr_lockss (map fst exs) l))"
+	  hence "lock_expr_locks_ok (locks s1 $ l) t 0 (int (expr_locks e l + expr_lockss (map fst exs) l))"
 	    by(simp add: lock_expr_locks_ok_def)
-	  with lao have "lock_expr_locks_ok (upd_locks ((locks s1)\<^sub>f l) t (\<lbrace>ta\<rbrace>\<^bsub>l\<^esub>\<^sub>f l)) t (upd_threadRs 0 ((locks s1)\<^sub>f l) t (\<lbrace>ta\<rbrace>\<^bsub>l\<^esub>\<^sub>f l))
- (upd_expr_lock_actions (int (expr_locks e l + expr_lockss (map fst exs) l)) (\<lbrace>ta\<rbrace>\<^bsub>l\<^esub>\<^sub>f l))"
+	  with lao have "lock_expr_locks_ok (upd_locks (locks s1 $ l) t (\<lbrace>ta\<rbrace>\<^bsub>l\<^esub> $ l)) t (upd_threadRs 0 (locks s1 $ l) t (\<lbrace>ta\<rbrace>\<^bsub>l\<^esub> $ l))
+ (upd_expr_lock_actions (int (expr_locks e l + expr_lockss (map fst exs) l)) (\<lbrace>ta\<rbrace>\<^bsub>l\<^esub> $ l))"
 	    by(rule upd_locks_upd_expr_lock_preserve_lock_expr_locks_ok)
 	  moreover from sync thrst x have "sync_ok e" "el_loc_ok e x"
 	    unfolding el_loc_ok1_def by(auto dest: ts_okD)
 	  with red1_update_expr_locks[OF wf red]
 	  have "upd_expr_locks (int \<circ> expr_locks e) \<lbrace>TA\<rbrace>\<^bsub>l\<^esub> = int \<circ> expr_locks e'" by(simp)
-	  hence "upd_expr_lock_actions (int (expr_locks e l)) (\<lbrace>TA\<rbrace>\<^bsub>l\<^esub>\<^sub>f l) = int (expr_locks e' l)"
+	  hence "upd_expr_lock_actions (int (expr_locks e l)) (\<lbrace>TA\<rbrace>\<^bsub>l\<^esub> $ l) = int (expr_locks e' l)"
 	    by(simp add: upd_expr_locks_def fun_eq_iff)
 	  ultimately show ?thesis using lao Some thrst x True
             by(auto simp add: lock_expr_locks_ok_def upd_expr_locks_def)
@@ -436,7 +436,7 @@ proof(cases rule: Red1_mthr.redT.cases)
 	      where nt: "NewThread t' (eX, eXS) m \<in> set (map (convert_new_thread_action (extNTA2J1 P)) \<lbrace>TA\<rbrace>\<^bsub>t\<^esub>)"
 	      and [simp]: "LN = no_wait_locks" by(auto dest: redT_updTs_new_thread)
 	    note expr_locks_new_thread1[OF wf red nt]
-	    moreover from loks True have "has_locks ((locks s1)\<^sub>f l) t' = 0"
+	    moreover from loks True have "has_locks (locks s1 $ l) t' = 0"
 	      by(force simp add: lock_oks1_def)
 	    ultimately show ?thesis using lao False by simp
 	  next
@@ -446,7 +446,7 @@ proof(cases rule: Red1_mthr.redT.cases)
 	    with loks tok lao `t \<noteq> t'` show ?thesis by(cases eX)(auto simp add: lock_oks1_def)
 	  qed
 	qed }
-      hence "\<forall>l. has_locks ((redT_updLs (locks s1) t \<lbrace>ta\<rbrace>\<^bsub>l\<^esub>)\<^sub>f l) t' + LN\<^sub>f l = expr_lockss (map fst (eX # eXS)) l" .. }
+      hence "\<forall>l. has_locks ((redT_updLs (locks s1) t \<lbrace>ta\<rbrace>\<^bsub>l\<^esub>) $ l) t' + LN $ l = expr_lockss (map fst (eX # eXS)) l" .. }
     ultimately show ?thesis using s1' unfolding lock_oks1_def x' by(clarsimp simp del: fun_upd_apply)
   next
     case (red1Call e a M vs U Ts T body D x)
@@ -481,7 +481,7 @@ next
   thus ?thesis using loks unfolding lock_oks1_def
     apply auto
      apply force
-    apply(case_tac "ln\<^sub>f l::nat")
+    apply(case_tac "ln $ l::nat")
      apply simp
      apply(erule allE)
      apply(erule conjE)
@@ -662,7 +662,7 @@ proof -
   from Red show ?thesis
   proof(cases)
     case (redT_acquire t x ln n)
-    hence "Red1_mthr.redT False P ?s1 (t, \<lambda>\<^isup>f [], [], [], [], [], convert_RA ln) ?s1'"
+    hence "Red1_mthr.redT False P ?s1 (t, K$ [], [], [], [], [], convert_RA ln) ?s1'"
       by(cases x)(auto intro!: Red1_mthr.redT.redT_acquire simp add: init_fin_descend_thr_def)
     with wf have "lock_oks1 (locks ?s1') (thr ?s1')" using loks' sync' by(rule Red1'_preserves_lock_oks)
     thus ?thesis by simp
