thys/JinjaThreads/Framework/FWLocking.thy
@@ -10,94 +10,94 @@ imports
 begin
 
 definition redT_updLs :: "('l,'t) locks \<Rightarrow> 't \<Rightarrow> 'l lock_actions \<Rightarrow> ('l,'t) locks" where
-  "redT_updLs ls t las \<equiv> (\<lambda>(l, la). upd_locks l t la) \<circ>\<^isub>f ((ls, las)\<^sup>f)"
+  "redT_updLs ls t las \<equiv> (\<lambda>(l, la). upd_locks l t la) \<circ>$ (($ls, las$))"
 
-lemma redT_updLs_iff [simp]: "(redT_updLs ls t las)\<^sub>f l = upd_locks (ls\<^sub>f l) t (las\<^sub>f l)"
+lemma redT_updLs_iff [simp]: "redT_updLs ls t las $ l = upd_locks (ls $ l) t (las $ l)"
 by(simp add: redT_updLs_def)
 
-lemma upd_locks_empty_conv [simp]: "(\<lambda>(l, las). upd_locks l t las) \<circ>\<^isub>f (ls, \<lambda>\<^isup>f [])\<^sup>f = ls"
+lemma upd_locks_empty_conv [simp]: "(\<lambda>(l, las). upd_locks l t las) \<circ>$ ($ls, K$ []$) = ls"
 by(auto intro: finfun_ext)
 
 lemma redT_updLs_Some_thread_idD:
-  "\<lbrakk> has_lock ((redT_updLs ls t las)\<^sub>f l) t'; t \<noteq> t' \<rbrakk> \<Longrightarrow> has_lock (ls\<^sub>f l) t'"
+  "\<lbrakk> has_lock (redT_updLs ls t las $ l) t'; t \<noteq> t' \<rbrakk> \<Longrightarrow> has_lock (ls $ l) t'"
 by(auto simp add: redT_updLs_def intro: has_lock_upd_locks_implies_has_lock)
 
-definition acquire_all :: "('l, 't) locks \<Rightarrow> 't \<Rightarrow> ('l \<Rightarrow>\<^isub>f nat) \<Rightarrow> ('l, 't) locks"
-where "acquire_all ls t ln \<equiv> (\<lambda>(l, la). acquire_locks l t la) \<circ>\<^isub>f ((ls, ln)\<^sup>f)"
+definition acquire_all :: "('l, 't) locks \<Rightarrow> 't \<Rightarrow> ('l \<Rightarrow>f nat) \<Rightarrow> ('l, 't) locks"
+where "acquire_all ls t ln \<equiv> (\<lambda>(l, la). acquire_locks l t la) \<circ>$ (($ls, ln$))"
 
 lemma acquire_all_iff [simp]: 
-  "(acquire_all ls t ln)\<^sub>f l = acquire_locks (ls\<^sub>f l) t (ln\<^sub>f l)"
+  "acquire_all ls t ln $ l = acquire_locks (ls $ l) t (ln $ l)"
 by(simp add: acquire_all_def)
 
 
 definition lock_ok_las :: "('l,'t) locks \<Rightarrow> 't \<Rightarrow> 'l lock_actions \<Rightarrow> bool" where
-  "lock_ok_las ls t las \<equiv> \<forall>l. lock_actions_ok (ls\<^sub>f l) t (las\<^sub>f l)"
+  "lock_ok_las ls t las \<equiv> \<forall>l. lock_actions_ok (ls $ l) t (las $ l)"
 
 lemma lock_ok_lasI [intro]:
-  "(\<And>l. lock_actions_ok (ls\<^sub>f l) t (las\<^sub>f l)) \<Longrightarrow> lock_ok_las ls t las"
+  "(\<And>l. lock_actions_ok (ls $ l) t (las $ l)) \<Longrightarrow> lock_ok_las ls t las"
 by(simp add: lock_ok_las_def)
 
 lemma lock_ok_lasE:
-  "\<lbrakk> lock_ok_las ls t las; (\<And>l. lock_actions_ok (ls\<^sub>f l) t (las\<^sub>f l)) \<Longrightarrow> Q \<rbrakk> \<Longrightarrow> Q"
+  "\<lbrakk> lock_ok_las ls t las; (\<And>l. lock_actions_ok (ls $ l) t (las $ l)) \<Longrightarrow> Q \<rbrakk> \<Longrightarrow> Q"
 by(simp add: lock_ok_las_def)
 
 lemma lock_ok_lasD:
-  "lock_ok_las ls t las \<Longrightarrow> lock_actions_ok (ls\<^sub>f l) t (las\<^sub>f l)"
+  "lock_ok_las ls t las \<Longrightarrow> lock_actions_ok (ls $ l) t (las $ l)"
 by(simp add: lock_ok_las_def)
 
 lemma lock_ok_las_code [code]:
-  "lock_ok_las ls t las = finfun_All ((\<lambda>(l, la). lock_actions_ok l t la) \<circ>\<^isub>f (ls, las)\<^sup>f)"
+  "lock_ok_las ls t las = finfun_All ((\<lambda>(l, la). lock_actions_ok l t la) \<circ>$ ($ls, las$))"
 by(simp add: lock_ok_las_def finfun_All_All o_def)
 
 lemma lock_ok_las_may_lock:
-  "\<lbrakk> lock_ok_las ls t las; Lock \<in> set (las\<^sub>f l) \<rbrakk> \<Longrightarrow> may_lock (ls\<^sub>f l) t"
+  "\<lbrakk> lock_ok_las ls t las; Lock \<in> set (las $ l) \<rbrakk> \<Longrightarrow> may_lock (ls $ l) t"
 by(erule lock_ok_lasE)(rule lock_actions_ok_Lock_may_lock)
 
 lemma redT_updLs_may_lock [simp]:
-  "lock_ok_las ls t las \<Longrightarrow> may_lock ((redT_updLs ls t las)\<^sub>f l) t = may_lock (ls\<^sub>f l) t"
+  "lock_ok_las ls t las \<Longrightarrow> may_lock (redT_updLs ls t las $ l) t = may_lock (ls $ l) t"
 by(auto dest!: lock_ok_lasD[where l=l])
 
 lemma redT_updLs_has_locks [simp]:
-  "\<lbrakk> lock_ok_las ls t' las; t \<noteq> t' \<rbrakk> \<Longrightarrow> has_locks ((redT_updLs ls t' las)\<^sub>f l) t = has_locks (ls\<^sub>f l) t"
+  "\<lbrakk> lock_ok_las ls t' las; t \<noteq> t' \<rbrakk> \<Longrightarrow> has_locks (redT_updLs ls t' las $ l) t = has_locks (ls $ l) t"
 by(auto dest!: lock_ok_lasD[where l=l])
 
 
-definition may_acquire_all :: "('l, 't) locks \<Rightarrow> 't \<Rightarrow> ('l \<Rightarrow>\<^isub>f nat) \<Rightarrow> bool"
-where "may_acquire_all ls t ln \<equiv> \<forall>l. ln\<^sub>f l > 0 \<longrightarrow> may_lock (ls\<^sub>f l) t"
+definition may_acquire_all :: "('l, 't) locks \<Rightarrow> 't \<Rightarrow> ('l \<Rightarrow>f nat) \<Rightarrow> bool"
+where "may_acquire_all ls t ln \<equiv> \<forall>l. ln $ l > 0 \<longrightarrow> may_lock (ls $ l) t"
 
 lemma may_acquire_allI [intro]:
-  "(\<And>l. ln\<^sub>f l > 0 \<Longrightarrow> may_lock (ls\<^sub>f l) t) \<Longrightarrow> may_acquire_all ls t ln"
+  "(\<And>l. ln $ l > 0 \<Longrightarrow> may_lock (ls $ l) t) \<Longrightarrow> may_acquire_all ls t ln"
 by(simp add: may_acquire_all_def)
 
 lemma may_acquire_allE:
-  "\<lbrakk> may_acquire_all ls t ln; \<forall>l. ln\<^sub>f l > 0 \<longrightarrow> may_lock (ls\<^sub>f l) t \<Longrightarrow> P \<rbrakk> \<Longrightarrow> P"
+  "\<lbrakk> may_acquire_all ls t ln; \<forall>l. ln $ l > 0 \<longrightarrow> may_lock (ls $ l) t \<Longrightarrow> P \<rbrakk> \<Longrightarrow> P"
 by(auto simp add: may_acquire_all_def)
 
 lemma may_acquire_allD [dest]:
-  "\<lbrakk> may_acquire_all ls t ln; ln\<^sub>f l > 0 \<rbrakk> \<Longrightarrow> may_lock (ls\<^sub>f l) t"
+  "\<lbrakk> may_acquire_all ls t ln; ln $ l > 0 \<rbrakk> \<Longrightarrow> may_lock (ls $ l) t"
 by(auto simp add: may_acquire_all_def)
 
 lemma may_acquire_all_has_locks_acquire_locks [simp]:
-  "\<lbrakk> may_acquire_all ls t ln; t \<noteq> t' \<rbrakk> \<Longrightarrow> has_locks (acquire_locks (ls\<^sub>f l) t (ln\<^sub>f l)) t' = has_locks (ls\<^sub>f l) t'"
-by(cases "ln\<^sub>f l > 0")(auto dest: may_acquire_allD)
+  "\<lbrakk> may_acquire_all ls t ln; t \<noteq> t' \<rbrakk> \<Longrightarrow> has_locks (acquire_locks (ls $ l) t (ln $ l)) t' = has_locks (ls $ l) t'"
+by(cases "ln $ l > 0")(auto dest: may_acquire_allD)
 
 lemma may_acquire_all_code [code]:
-  "may_acquire_all ls t ln \<longleftrightarrow> finfun_All ((\<lambda>(lock, n). n > 0 \<longrightarrow> may_lock lock t) \<circ>\<^isub>f (ls, ln)\<^sup>f)"
+  "may_acquire_all ls t ln \<longleftrightarrow> finfun_All ((\<lambda>(lock, n). n > 0 \<longrightarrow> may_lock lock t) \<circ>$ ($ls, ln$))"
 by(auto simp add: may_acquire_all_def finfun_All_All o_def)
 
 definition collect_locks :: "'l lock_actions \<Rightarrow> 'l set" where
-  "collect_locks las = {l. Lock \<in> set (las\<^sub>f l)}"
+  "collect_locks las = {l. Lock \<in> set (las $ l)}"
 
 lemma collect_locksI:
-  "Lock \<in> set (las\<^sub>f l) \<Longrightarrow> l \<in> collect_locks las"
+  "Lock \<in> set (las $ l) \<Longrightarrow> l \<in> collect_locks las"
 by(simp add: collect_locks_def)
 
 lemma collect_locksE:
-  "\<lbrakk> l \<in> collect_locks las; Lock \<in> set (las\<^sub>f l) \<Longrightarrow> P \<rbrakk> \<Longrightarrow> P"
+  "\<lbrakk> l \<in> collect_locks las; Lock \<in> set (las $ l) \<Longrightarrow> P \<rbrakk> \<Longrightarrow> P"
 by(simp add: collect_locks_def)
 
 lemma collect_locksD:
-  "l \<in> collect_locks las \<Longrightarrow> Lock \<in> set (las\<^sub>f l)"
+  "l \<in> collect_locks las \<Longrightarrow> Lock \<in> set (las $ l)"
 by(simp add: collect_locks_def)
 
 
@@ -123,7 +123,7 @@ proof(induct las)
 qed simp
 
 lemma must_acquire_lock_conv:
-  "must_acquire_lock las = (case (filter (\<lambda>L. L = Lock \<or> L = Unlock) las) of [] \<Rightarrow> False | L#Ls \<Rightarrow> L = Lock)"
+  "must_acquire_lock las = (case (filter (\<lambda>L. L = Lock \<or> L = Unlock) las) of [] \<Rightarrow> False | L # Ls \<Rightarrow> L = Lock)"
 proof(induct las)
   case Nil thus ?case by simp
 next
@@ -133,14 +133,14 @@ qed
 
 
 definition collect_locks' :: "'l lock_actions \<Rightarrow> 'l set" where
-  "collect_locks' las \<equiv> {l. must_acquire_lock (las\<^sub>f l)}"
+  "collect_locks' las \<equiv> {l. must_acquire_lock (las $ l)}"
 
 lemma collect_locks'I:
-  "must_acquire_lock (las\<^sub>f l) \<Longrightarrow> l \<in> collect_locks' las"
+  "must_acquire_lock (las $ l) \<Longrightarrow> l \<in> collect_locks' las"
 by(simp add: collect_locks'_def)
 
 lemma collect_locks'E:
-  "\<lbrakk> l \<in> collect_locks' las; must_acquire_lock (las\<^sub>f l) \<Longrightarrow> P \<rbrakk> \<Longrightarrow> P"
+  "\<lbrakk> l \<in> collect_locks' las; must_acquire_lock (las $ l) \<Longrightarrow> P \<rbrakk> \<Longrightarrow> P"
 by(simp add: collect_locks'_def)
 
 lemma collect_locks'_subset_collect_locks:
@@ -148,41 +148,41 @@ lemma collect_locks'_subset_collect_locks:
 by(auto simp add: collect_locks'_def collect_locks_def intro: must_acquire_lock_contains_lock)
 
 definition lock_ok_las' :: "('l,'t) locks \<Rightarrow> 't \<Rightarrow> 'l lock_actions \<Rightarrow> bool" where
-  "lock_ok_las' ls t las \<equiv> \<forall>l. lock_actions_ok' (ls\<^sub>f l) t (las\<^sub>f l)"
+  "lock_ok_las' ls t las \<equiv> \<forall>l. lock_actions_ok' (ls $ l) t (las $ l)"
 
-lemma lock_ok_las'I: "(\<And>l. lock_actions_ok' (ls\<^sub>f l) t (las\<^sub>f l)) \<Longrightarrow> lock_ok_las' ls t las"
+lemma lock_ok_las'I: "(\<And>l. lock_actions_ok' (ls $ l) t (las $ l)) \<Longrightarrow> lock_ok_las' ls t las"
 by(simp add: lock_ok_las'_def)
 
-lemma lock_ok_las'D: "lock_ok_las' ls t las \<Longrightarrow> lock_actions_ok' (ls\<^sub>f l) t (las\<^sub>f l)"
+lemma lock_ok_las'D: "lock_ok_las' ls t las \<Longrightarrow> lock_actions_ok' (ls $ l) t (las $ l)"
 by(simp add: lock_ok_las'_def)
 
 lemma not_lock_ok_las'_conv:
-  "\<not> lock_ok_las' ls t las \<longleftrightarrow> (\<exists>l. \<not> lock_actions_ok' (ls\<^sub>f l) t (las\<^sub>f l))"
+  "\<not> lock_ok_las' ls t las \<longleftrightarrow> (\<exists>l. \<not> lock_actions_ok' (ls $ l) t (las $ l))"
 by(simp add: lock_ok_las'_def)
 
 lemma lock_ok_las'_code:
-    "lock_ok_las' ls t las = finfun_All ((\<lambda>(l, la). lock_actions_ok' l t la) \<circ>\<^isub>f (ls, las)\<^sup>f)"
+    "lock_ok_las' ls t las = finfun_All ((\<lambda>(l, la). lock_actions_ok' l t la) \<circ>$ ($ls, las$))"
 by(simp add: lock_ok_las'_def finfun_All_All o_def)
 
 
 lemma lock_ok_las'_collect_locks'_may_lock:
   assumes lot': "lock_ok_las' ls t las"
-  and mayl: "\<forall>l \<in> collect_locks' las. may_lock (ls\<^sub>f l) t"
+  and mayl: "\<forall>l \<in> collect_locks' las. may_lock (ls $ l) t"
   and l: "l \<in> collect_locks las"
-  shows "may_lock (ls\<^sub>f l) t"
+  shows "may_lock (ls $ l) t"
 proof(cases "l \<in> collect_locks' las")
   case True thus ?thesis using mayl by auto
 next
   case False
-  hence nmal: "\<not> must_acquire_lock (las\<^sub>f l)"
+  hence nmal: "\<not> must_acquire_lock (las $ l)"
     by(auto intro: collect_locks'I)
-  from l have locklasl: "Lock \<in> set (las\<^sub>f l)"
+  from l have locklasl: "Lock \<in> set (las $ l)"
     by(rule collect_locksD)
   then obtain ys zs
-    where las: "las\<^sub>f l = ys @ Lock # zs"
+    where las: "las $ l = ys @ Lock # zs"
     and notin: "Lock \<notin> set ys"
     by(auto dest: split_list_first)
-  from lot' have "lock_actions_ok' (ls\<^sub>f l) t (las\<^sub>f l)"
+  from lot' have "lock_actions_ok' (ls $ l) t (las $ l)"
     by(auto simp add: lock_ok_las'_def)
   thus ?thesis
   proof(induct rule: lock_actions_ok'E)
@@ -191,20 +191,20 @@ next
       by -(rule lock_actions_ok_Lock_may_lock)
   next
     case (Lock YS ZS)
-    note LAS = `las\<^sub>f l = YS @ Lock # ZS`
-    note lao = `lock_actions_ok (ls\<^sub>f l) t YS`
-    note nml = `\<not> may_lock (upd_locks (ls\<^sub>f l) t YS) t`
+    note LAS = `las $ l = YS @ Lock # ZS`
+    note lao = `lock_actions_ok (ls $ l) t YS`
+    note nml = `\<not> may_lock (upd_locks (ls $ l) t YS) t`
     from LAS las nmal notin have "Unlock \<in> set YS"
       by -(erule contrapos_np, auto simp add: must_acquire_lock_append append_eq_append_conv2 append_eq_Cons_conv)
     then obtain ys' zs'
       where YS: "YS = ys' @ Unlock # zs'"
       and unlock: "Unlock \<notin> set ys'"
       by(auto dest: split_list_first)
-    from YS las LAS lao have lao': "lock_actions_ok (ls\<^sub>f l) t (ys' @ [Unlock])" by(auto)
-    hence "has_lock (upd_locks (ls\<^sub>f l) t ys') t" by simp
-    hence "may_lock (upd_locks (ls\<^sub>f l) t ys') t"
+    from YS las LAS lao have lao': "lock_actions_ok (ls $ l) t (ys' @ [Unlock])" by(auto)
+    hence "has_lock (upd_locks (ls $ l) t ys') t" by simp
+    hence "may_lock (upd_locks (ls $ l) t ys') t"
       by(rule has_lock_may_lock)
-    moreover from lao' have "lock_actions_ok (ls\<^sub>f l) t ys'" by simp
+    moreover from lao' have "lock_actions_ok (ls $ l) t ys'" by simp
     ultimately show ?thesis by simp
   qed
 qed
@@ -223,21 +223,21 @@ qed
 
 lemma lock_ok_las'_collect_locks_lock_ok_las:
   assumes lol': "lock_ok_las' ls t las"
-  and clml: "\<And>l. l \<in> collect_locks las \<Longrightarrow> may_lock (ls\<^sub>f l) t"
+  and clml: "\<And>l. l \<in> collect_locks las \<Longrightarrow> may_lock (ls $ l) t"
   shows "lock_ok_las ls t las"
 proof(rule lock_ok_lasI)
   fix l
-  from lol' have "lock_actions_ok' (ls\<^sub>f l) t (las\<^sub>f l)" by(rule lock_ok_las'D)
-  thus "lock_actions_ok (ls\<^sub>f l) t (las\<^sub>f l)"
+  from lol' have "lock_actions_ok' (ls $ l) t (las $ l)" by(rule lock_ok_las'D)
+  thus "lock_actions_ok (ls $ l) t (las $ l)"
   proof(rule lock_actions_ok'_must_acquire_lock_lock_actions_ok[OF _ impI])
-    assume mal: "must_acquire_lock (las\<^sub>f l)"
-    thus "may_lock (ls\<^sub>f l) t"
+    assume mal: "must_acquire_lock (las $ l)"
+    thus "may_lock (ls $ l) t"
       by(auto intro!: clml collect_locksI elim: must_acquire_lock_contains_lock )
   qed
 qed
 
 lemma lock_ok_las'_into_lock_on_las:
-  "\<lbrakk>lock_ok_las' ls t las; \<And>l. l \<in> collect_locks' las \<Longrightarrow> may_lock (ls\<^sub>f l) t\<rbrakk> \<Longrightarrow> lock_ok_las ls t las"
+  "\<lbrakk>lock_ok_las' ls t las; \<And>l. l \<in> collect_locks' las \<Longrightarrow> may_lock (ls $ l) t\<rbrakk> \<Longrightarrow> lock_ok_las ls t las"
 by (metis lock_ok_las'_collect_locks'_may_lock lock_ok_las'_collect_locks_lock_ok_las)
 
 end
