thys/JinjaThreads/Basic/Aux.thy
@@ -11,7 +11,7 @@ header {*
 theory Aux 
 imports
   Main
-  "../../FinFun/FinFun"
+  "~~/src/HOL/Library/FinFun_Syntax"
   "~~/src/HOL/Library/Transitive_Closure_Table"
   "~~/src/HOL/Library/Predicate_Compile_Alternative_Defs"
   "~~/src/HOL/Library/Code_Char"
