thys/JinjaThreads/Common/ExternalCallWF.thy
@@ -489,10 +489,10 @@ proof(atomize_elim)
       next
         case RedWaitInterrupt
         note ta = `ta = \<lbrace>Unlock\<rightarrow>a, Lock\<rightarrow>a, IsInterrupted t True, ClearInterrupt t, ObsInterrupted t\<rbrace>`
-        from ta False None have hli: "\<not> has_lock ((locks s)\<^sub>f a) t \<or> t \<notin> interrupts s"
+        from ta False None have hli: "\<not> has_lock (locks s $ a) t \<or> t \<notin> interrupts s"
           by(fastforce simp add: lock_actions_ok'_iff finfun_upd_apply split: split_if_asm dest: may_lock_t_may_lock_unlock_lock_t dest: has_lock_may_lock)
         show ?thesis
-        proof(cases "has_lock ((locks s)\<^sub>f a) t")
+        proof(cases "has_lock (locks s $ a) t")
           case True
           let ?ta' = "\<lbrace>Suspend a, Unlock\<rightarrow>a, Lock\<rightarrow>a, ReleaseAcquire\<rightarrow>a, IsInterrupted t False, SyncUnlock a \<rbrace>"
           from True hli have "t \<notin> interrupts s" by simp
@@ -516,10 +516,10 @@ proof(atomize_elim)
         case RedWait
         note ta = `ta = \<lbrace>Suspend a, Unlock\<rightarrow>a, Lock\<rightarrow>a, ReleaseAcquire\<rightarrow>a, IsInterrupted t False, SyncUnlock a\<rbrace>`
 
-        from ta False None have hli: "\<not> has_lock ((locks s)\<^sub>f a) t \<or> t \<in> interrupts s"
+        from ta False None have hli: "\<not> has_lock (locks s $ a) t \<or> t \<in> interrupts s"
           by(auto simp add: lock_actions_ok'_iff finfun_upd_apply wset_actions_ok_def Cons_eq_append_conv split: split_if_asm dest: may_lock_t_may_lock_unlock_lock_t dest: has_lock_may_lock)
         show ?thesis
-        proof(cases "has_lock ((locks s)\<^sub>f a) t")
+        proof(cases "has_lock (locks s $ a) t")
           case True
           let ?ta' = "\<lbrace>Unlock\<rightarrow>a, Lock\<rightarrow>a, IsInterrupted t True, ClearInterrupt t, ObsInterrupted t\<rbrace>"
           from True hli have "t \<in> interrupts s" by simp
@@ -543,7 +543,7 @@ proof(atomize_elim)
         let ?ta' = "if t \<in> interrupts s
                    then \<lbrace>Unlock\<rightarrow>a, Lock\<rightarrow>a, IsInterrupted t True, ClearInterrupt t, ObsInterrupted t\<rbrace>
                    else \<lbrace>Suspend a, Unlock\<rightarrow>a, Lock\<rightarrow>a, ReleaseAcquire\<rightarrow>a, IsInterrupted t False, SyncUnlock a \<rbrace>"
-        from ta False None have "has_lock ((locks s)\<^sub>f a) t"
+        from ta False None have "has_lock (locks s $ a) t"
           by(auto simp add: finfun_upd_apply split: split_if_asm)
         hence "final_thread.actions_ok final s t ?ta'" using None
           by(auto simp add: final_thread.actions_ok_iff final_thread.cond_action_oks.simps lock_ok_las_def finfun_upd_apply has_lock_may_lock wset_actions_ok_def)
@@ -554,7 +554,7 @@ proof(atomize_elim)
       next
         case RedWaitNotified
         note ta = `ta = \<lbrace>Notified\<rbrace>`
-        let ?ta' = "if has_lock ((locks s)\<^sub>f a) t
+        let ?ta' = "if has_lock (locks s $ a) t
                    then (if t \<in> interrupts s 
                          then \<lbrace>Unlock\<rightarrow>a, Lock\<rightarrow>a, IsInterrupted t True, ClearInterrupt t, ObsInterrupted t\<rbrace>
                          else \<lbrace>Suspend a, Unlock\<rightarrow>a, Lock\<rightarrow>a, ReleaseAcquire\<rightarrow>a, IsInterrupted t False, SyncUnlock a \<rbrace>)
@@ -567,7 +567,7 @@ proof(atomize_elim)
       next
         case RedWaitInterrupted
         note ta = `ta = \<lbrace>WokenUp, ClearInterrupt t, ObsInterrupted t\<rbrace>`
-        let ?ta' = "if has_lock ((locks s)\<^sub>f a) t
+        let ?ta' = "if has_lock (locks s $ a) t
                    then (if t \<in> interrupts s 
                          then \<lbrace>Unlock\<rightarrow>a, Lock\<rightarrow>a, IsInterrupted t True, ClearInterrupt t, ObsInterrupted t\<rbrace>
                          else \<lbrace>Suspend a, Unlock\<rightarrow>a, Lock\<rightarrow>a, ReleaseAcquire\<rightarrow>a, IsInterrupted t False, SyncUnlock a \<rbrace>)
@@ -581,7 +581,7 @@ proof(atomize_elim)
         case RedNotify
         note ta = `ta = \<lbrace>Notify a, Unlock\<rightarrow>a, Lock\<rightarrow>a\<rbrace>`
         let ?ta' = "\<lbrace>UnlockFail\<rightarrow>a\<rbrace>"
-        from ta False None have "\<not> has_lock ((locks s)\<^sub>f a) t"
+        from ta False None have "\<not> has_lock (locks s $ a) t"
 	  by(fastforce simp add: lock_actions_ok'_iff finfun_upd_apply wset_actions_ok_def Cons_eq_append_conv split: split_if_asm dest: may_lock_t_may_lock_unlock_lock_t has_lock_may_lock)
         hence "final_thread.actions_ok' s t ?ta'" using None
           by(auto simp add: lock_actions_ok'_iff finfun_upd_apply)
@@ -593,7 +593,7 @@ proof(atomize_elim)
         case RedNotifyFail
         note ta = `ta = \<lbrace>UnlockFail\<rightarrow>a\<rbrace>`
         let ?ta' = "\<lbrace>Notify a, Unlock\<rightarrow>a, Lock\<rightarrow>a\<rbrace>"
-        from ta False None have "has_lock ((locks s)\<^sub>f a) t"
+        from ta False None have "has_lock (locks s $ a) t"
           by(auto simp add: finfun_upd_apply split: split_if_asm)
         hence "final_thread.actions_ok' s t ?ta'" using None
           by(auto simp add: finfun_upd_apply simp add: wset_actions_ok_def intro: has_lock_may_lock)
@@ -605,7 +605,7 @@ proof(atomize_elim)
         case RedNotifyAll
         note ta = `ta = \<lbrace>NotifyAll a, Unlock\<rightarrow>a, Lock\<rightarrow>a\<rbrace>`
         let ?ta' = "\<lbrace>UnlockFail\<rightarrow>a\<rbrace>"
-        from ta False None have "\<not> has_lock ((locks s)\<^sub>f a) t"
+        from ta False None have "\<not> has_lock (locks s $ a) t"
 	  by(auto simp add: lock_actions_ok'_iff finfun_upd_apply wset_actions_ok_def Cons_eq_append_conv split: split_if_asm dest: may_lock_t_may_lock_unlock_lock_t)
         hence "final_thread.actions_ok' s t ?ta'" using None
           by(auto simp add: lock_actions_ok'_iff finfun_upd_apply)
@@ -617,7 +617,7 @@ proof(atomize_elim)
         case RedNotifyAllFail
         note ta = `ta = \<lbrace>UnlockFail\<rightarrow>a\<rbrace>`
         let ?ta' = "\<lbrace>NotifyAll a, Unlock\<rightarrow>a, Lock\<rightarrow>a\<rbrace>"
-        from ta False None have "has_lock ((locks s)\<^sub>f a) t"
+        from ta False None have "has_lock (locks s $ a) t"
           by(auto simp add: finfun_upd_apply split: split_if_asm)
         hence "final_thread.actions_ok' s t ?ta'" using None
           by(auto simp add: finfun_upd_apply wset_actions_ok_def intro: has_lock_may_lock)
@@ -663,7 +663,7 @@ proof -
     free_thread_id.intros
     and [cong] = conj_cong
   
-  from assms show ?thesis by cases(fastforce intro: exI[where x="(\<lambda>\<^isup>f None)(\<^sup>f a := \<lfloor>(t, 0)\<rfloor>)"] exI[where x="(\<lambda>\<^isup>f None)"])+
+  from assms show ?thesis by cases(fastforce intro: exI[where x="(K$ None)(a $:= \<lfloor>(t, 0)\<rfloor>)"] exI[where x="(K$ None)"])+
 qed
 
 lemma red_external_aggr_ta_satisfiable:
@@ -679,7 +679,7 @@ proof -
     and [cong] = conj_cong
   
   from assms show ?thesis
-    by(fastforce simp add: red_external_aggr_def split_beta ta_upd_simps split: split_if_asm intro: exI[where x="empty"] exI[where x="(\<lambda>\<^isup>f None)(\<^sup>f a := \<lfloor>(t, 0)\<rfloor>)"] exI[where x="(\<lambda>\<^isup>f None)"])
+    by(fastforce simp add: red_external_aggr_def split_beta ta_upd_simps split: split_if_asm intro: exI[where x="empty"] exI[where x="(K$ None)(a $:= \<lfloor>(t, 0)\<rfloor>)"] exI[where x="K$ None"])
 qed
 
 end
