thys/JinjaThreads/Execute/SC_Schedulers.thy
@@ -19,7 +19,7 @@ where
    heap_base.start_state_refine addr2thread_id sc_empty (sc_allocate P) thr_empty thr_update ws_empty is_empty f P"
 
 abbreviation sc_state_\<alpha> ::
-  "('l, 't :: linorder, 'm, ('t, 'x \<times> 'l \<Rightarrow>\<^isub>f nat) rm, ('t, 'w wait_set_status) rm, 't rs) state_refine
+  "('l, 't :: linorder, 'm, ('t, 'x \<times> 'l \<Rightarrow>f nat) rm, ('t, 'w wait_set_status) rm, 't rs) state_refine
   \<Rightarrow> ('l,'t,'x,'m,'w) state"
 where "sc_state_\<alpha> \<equiv> state_refine_base.state_\<alpha> rm_\<alpha> rm_\<alpha> rs_\<alpha>"
 
@@ -38,7 +38,7 @@ locale sc_scheduler =
   for final :: "'x \<Rightarrow> bool"
   and r :: "'t \<Rightarrow> ('x \<times> 'm) \<Rightarrow> (('l,'t :: linorder,'x,'m,'w,'o) thread_action \<times> 'x \<times> 'm) Predicate.pred"
   and convert_RA :: "'l released_locks \<Rightarrow> 'o list"
-  and schedule :: "('l,'t,'x,'m,'w,'o,('t, 'x \<times> 'l \<Rightarrow>\<^isub>f nat) rm,('t, 'w wait_set_status) rm, 't rs, 's) scheduler"
+  and schedule :: "('l,'t,'x,'m,'w,'o,('t, 'x \<times> 'l \<Rightarrow>f nat) rm,('t, 'w wait_set_status) rm, 't rs, 's) scheduler"
   and "output" :: "'s \<Rightarrow> 't \<Rightarrow> ('l,'t,'x,'m,'w,'o) thread_action \<Rightarrow> 'q option"
   and pick_wakeup :: "'s \<Rightarrow> 't \<Rightarrow> 'w \<Rightarrow> ('t, 'w wait_set_status) RBT.rbt \<Rightarrow> 't option"
   and \<sigma>_invar :: "'s \<Rightarrow> 't set \<Rightarrow> bool"
