thys/JinjaThreads/Framework/FWBisimulation.thy
@@ -1338,16 +1338,16 @@ proof -
     qed
   next
     case (redT_acquire x1 ln n)
-    hence [simp]: "ta1 = (\<lambda>\<^isup>f [], [], [], [], [], convert_RA ln)"
+    hence [simp]: "ta1 = (K$ [], [], [], [], [], convert_RA ln)"
       and tst: "thr s1 t = \<lfloor>(x1, ln)\<rfloor>" and wst: "\<not> waiting (wset s1 t)"
-      and maa: "may_acquire_all (locks s1) t ln" and ln: "0 < ln\<^sub>f n"
+      and maa: "may_acquire_all (locks s1) t ln" and ln: "0 < ln $ n"
       and s1': "s1' = (acquire_all ls1 t ln, (ts1(t \<mapsto> (x1, no_wait_locks)), m1), ws1, is1)" by auto
     from tst mbisim obtain x2 where tst': "ts2 t = \<lfloor>(x2, ln)\<rfloor>" 
       and bisim: "t \<turnstile> (x1, m1) \<approx> (x2, m2)" by(auto dest: mbisim_thrD1)
     let ?s2' = "(acquire_all ls1 t ln, (ts2(t \<mapsto> (x2, no_wait_locks)), m2), ws1, is1)"
-    from tst' wst maa ln have "s2 -2-t\<triangleright>(\<lambda>\<^isup>f [], [], [], [], [], convert_RA ln)\<rightarrow> ?s2'"
+    from tst' wst maa ln have "s2 -2-t\<triangleright>(K$ [], [], [], [], [], convert_RA ln)\<rightarrow> ?s2'"
       by-(rule r2.redT.redT_acquire, auto)
-    moreover from tst' ln have "\<not> m\<tau>move2 s2 (t, (\<lambda>\<^isup>f [], [], [], [], [], convert_RA ln)) ?s2'"
+    moreover from tst' ln have "\<not> m\<tau>move2 s2 (t, (K$ [], [], [], [], [], convert_RA ln)) ?s2'"
       by(auto simp add: acquire_all_def fun_eq_iff elim!: r2.m\<tau>move.cases)
     moreover have "mbisim s1' ?s2'"
     proof(rule mbisimI)
@@ -1382,7 +1382,7 @@ proof -
       from mbisim_wset_thread_ok1[OF mbisim]
       show "wset_thread_ok (wset s1') (thr s1')" using s1' by(auto intro: wset_thread_ok_upd)
     qed
-    moreover have "(t, \<lambda>\<^isup>f [], [], [], [], [], convert_RA ln) \<sim>T (t, \<lambda>\<^isup>f [], [], [], [], [], convert_RA ln)"
+    moreover have "(t, K$ [], [], [], [], [], convert_RA ln) \<sim>T (t, K$ [], [], [], [], [], convert_RA ln)"
       by(simp add: ta_bisim_def)
     ultimately show ?thesis by fastforce
   qed
